src/Node.v
@@ -1,0 +1,45 @@
+From Coq Require Import Init.Nat.
+From Coq Require Import Strings.String.
+
+Definition eqb_string (x y : string) : bool :=
+  if string_dec x y then true else false.
+
+Inductive node : Type :=
+  | Null
+  | Const (c : nat)
+  | Var (s : string).
+
+Definition is_const (n : node) : bool :=
+  (match n with
+   | Const _ => true
+   | otherwise => false
+   end).
+
+Definition is_var (n : node) : bool :=
+  (match n with
+   | Var _ => true
+   | otherwise => false
+   end).
+
+Check (Const 5) : node.
+Check (Var "x") : node.
+Check (Null) : node.
+
+Definition eqb_node (n1 n2 : node) : bool :=
+  (match n1, n2 with
+   | (Null), (Null) => true
+   | (Const c1), (Const c2) => c1 =? c2
+   | (Var s1),(Var s2) => eqb s1 s2
+   | e1,e2 => false
+   end).
+
+Example eqb_null_node :  eqb_node (Null) (Null) = true.
+Proof. reflexivity. Qed.
+Example eqb_const_eq_node:  eqb_node (Const 5) (Const 5) = true.
+Proof. reflexivity. Qed.
+Example eqb_const_neq_node:  eqb_node (Const 5) (Const 0) = false.
+Proof. reflexivity. Qed.
+Example eqb_var_eq_node :  eqb_node (Var "x") (Var "x") = true.
+Proof. reflexivity. Qed.
+Example eqb_var_neq_node :  eqb_node (Var "x") (Var "y") = false.
+Proof. reflexivity. Qed.
